Algorithms/inversions.dfy
@@ -13,432 +13,300 @@ module Inversions {
     }
 
     //{:vcs_split_on_every_assert}
-
-    // {
-    //     var x :| x in multiset(xs) && x in multiset(ys) && x in xs && x in ys;
-    // }
-
-
-
-    lemma {:verify } {:vcs_split_on_every_assert} JoinedWithMS(xs: seq<int>, ys: seq<int>, k: int, i: int)
-        requires xs != []
-        requires 0 <= k < |xs|
-        requires 0 <= i < |ys|
-        ensures IsInverted(xs+ys, k, |xs|+i) ==> JoinedWith(xs, ys, k) == JoinedWith(xs, ys[0..i] + ys[i+1..], k) + {(k, |xs|+i)}
-        ensures !IsInverted(xs+ys, k, |xs|+i) ==> JoinedWith(xs, ys, k) == JoinedWith(xs, ys[0..i] + ys[i+1..], k)
+    lemma PiecesEqual(xs: seq<int>, ys: seq<int>, sxs: seq<int>, sys: seq<int>, k: int)
+        requires multiset(xs) == multiset(sxs)
+        requires multiset(ys) == multiset(sys)
+        requires Sorted(sxs)
+        requires Sorted(sys)
+        requires |sxs| > 0
+        requires |sxs| == |xs|
+        requires 0 <= k < |xs| && xs[k] == sxs[0]
+        requires |inversersionSetJoined(xs[0..k] + xs[k+1..], ys)| == |inversersionSetJoined(sxs[1..], sys)|
+        ensures |pairKMap(inversersionSetJoined(xs[0..k] + xs[k+1..], ys), k, 1)| == |pairSetMap2(inversersionSetJoined(sxs[1..], sys), 1)|
     {
-        if ys == [] {
-        assert IsInverted(xs+ys, k, |xs|+i) ==> JoinedWith(xs, ys, k) == JoinedWith(xs, ys[0..i] + ys[i+1..], k) + {(k, |xs|+i)};
-        assert !IsInverted(xs+ys, k, |xs|+i) ==> JoinedWith(xs, ys, k) == JoinedWith(xs, ys[0..i] + ys[i+1..], k);
-        }else{
-            assert ys == ys[0..i]+[ys[i]]+ys[i+1..];
-            assert ys[i..] == [ys[i]]+ys[i+1..];
-            if IsInverted(xs+ys, k, |xs|+i) {
-                assert (xs+ys)[|xs|+i] == ys[i];
-                assert (xs+[ys[i]])[|xs|+0] == ys[i];
-                JoinedWithSplit(xs, ys, i, k);
-                assert |ys[i..]| > 0;
-                JoinedWithSplit(xs, ys[i..], 1, k);
-                assert JoinedWith(xs, [ys[i]], k) == {(k, |xs|)};
-                assert JoinedWith(xs, [ys[i]], k) !! pairSetRmap(JoinedWith(xs, ys[i+1..], k), 1) by {
-                    forall x | x in pairSetRmap(JoinedWith(xs, ys[i+1..], k), 1) 
-                        ensures x !in JoinedWith(xs, [ys[i]], k)
-                    {
-                        pairSetRmapInverse(JoinedWith(xs, ys[i+1..], k), 1, x);
-                        var pair := rmap(x, -1);
-                        assert pair in JoinedWith(xs, ys[i+1..], k);
-                        assert |xs| <= pair.1 < |xs|+|ys[i+1..]|;
-                        assert x.1 >= |xs|+1;
-                        // assert xs+ys[i+1..] < 
-                    }
-                }
-                calc {
-                    JoinedWith(xs, ys, k);
-                    JoinedWith(xs, ys[..i], k) + pairSetRmap(JoinedWith(xs, ys[i..], k), |ys[..i]|);
-                    JoinedWith(xs, ys[..i], k) + pairSetRmap(JoinedWith(xs, [ys[i]], k) + pairSetRmap(JoinedWith(xs, ys[i+1..], k), 1), |ys[..i]|);
-                    {pairSetRmapAdd(JoinedWith(xs, [ys[i]], k), pairSetRmap(JoinedWith(xs, ys[i+1..], k), 1) , |ys[..i]|);}
-                    JoinedWith(xs, ys[..i], k) + pairSetRmap(JoinedWith(xs, [ys[i]], k), |ys[..i]|) + pairSetRmap(pairSetRmap(JoinedWith(xs, ys[i+1..], k), 1), |ys[..i]|);
-                    {pairSetRmapNest(JoinedWith(xs, ys[i+1..], k),1,|ys[..i]|);}
-                    JoinedWith(xs, ys[..i], k) + pairSetRmap(JoinedWith(xs, [ys[i]], k), |ys[..i]|) + pairSetRmap(JoinedWith(xs, ys[i+1..], k), 1 + |ys[..i]|);
-                }
-                assert JoinedWith(xs, ys, k) == JoinedWith(xs, ys[0..i] + ys[i+1..], k) + {(k, |xs|+i)};
-            }else{
-                assert JoinedWith(xs, ys, k) == JoinedWith(xs, ys[0..i] + ys[i+1..], k);
+        pairSetMap2Lemma(inversersionSetJoined(sxs[1..], sys),1);
+        pairKMapSize(inversersionSetJoined(xs[0..k] + xs[k+1..], ys), k, 1);
+    }
+
+    lemma  inversetConcatOrderedUnorderedSame(xs: seq<int>, ys: seq<int>, sxs: seq<int>, sys: seq<int>)
+        requires multiset(xs) == multiset(sxs)
+        requires multiset(ys) == multiset(sys)
+        requires Sorted(sxs)
+        requires Sorted(sys)
+        ensures |inversersionSetJoined(xs, ys)| == |inversersionSetJoined(sxs, sys)|
+    {
+        var n := |xs| + |ys|;
+        var xsys := xs + ys;
+        assert |xsys| == n;
+        var sxsys := sxs + sys;
+        seqMsLength(xs, sxs);
+        seqMsLength(ys, sys);
+        assert |sxsys| == n;
+        assert multiset(xsys) == multiset(sxsys);
+        var invs := inversersionSetJoined(xs, ys);
+        if sxs == [] {
+            assert xs == [];
+            assert inversersionSetJoined(xs, ys) == {};
+            assert |inversersionSetJoined(xs, ys)| == 0;
+            assert |inversersionSetJoined(xs, ys)| == |inversersionSetJoined(sxs, sys)|;
+        }else {
+            assert |sxs| > 0;
+            var x := sxs[0];
+            assert sxs == [x] + sxs[1..];
+            assert x in multiset(xs);
+            var k :| 0 <= k < |xs| && x == xs[k];
+            assert xs == xs[0..k] + [x] + xs[k+1..];
+            assert multiset(xs) == multiset(xs[0..k] + [x] + xs[k+1..]);
+            calc {
+                multiset(sxs[1..]);
+                multiset(sxs)-multiset{x};
+                multiset(xs)-multiset{x};
+                multiset(xs[0..k] + xs[k+1..]);
             }
+            assert multiset(xs[0..k] + xs[k+1..]) == multiset(sxs[1..]);
+            inversetConcatOrderedUnorderedSame(xs[0..k] + xs[k+1..], ys, sxs[1..], sys);
+            assert |inversersionSetJoined(xs[0..k] + xs[k+1..], ys)| == |inversersionSetJoined(sxs[1..], sys)|;
+            var sortedInvs := inversersionSetJoined(sxs, sys);
+            var sxsFirst := JoinedWith(sxs, sys, 0);
+            inversersionSetJoinedFirsts(sxs, sys);
+            assert sxsFirst <= sortedInvs;
+            // assume sxsFirst !! pairSetMap2(inversersionSetJoined(sxs[1..], sys), 1);
+            assert sxsFirst + pairSetMap2(inversersionSetJoined(sxs[1..], sys),1) == inversersionSetJoined(sxs, sys);
+            assert sxsFirst !! pairSetMap2(inversersionSetJoined(sxs[1..], sys),1) by {
+                forall pair | pair in pairSetMap2(inversersionSetJoined(sxs[1..], sys), 1)
+                    ensures pair.0 != 0
+                {
+                    pairSetMap2Inverse(inversersionSetJoined(sxs[1..], sys), 1, pair);
+                }
+            }
+            assert pairSetMap2(inversersionSetJoined(sxs[1..], sys), 1) == inversersionSetJoined(sxs, sys) - sxsFirst;
+            var xsRest := JoinedWith(xs, ys, k);
+            inversionSetJoinedMiddle2(xs, ys, k);
+            assert xsRest + pairKMap(inversersionSetJoined(xs[0..k]+xs[k+1..], ys),k,1) == inversersionSetJoined(xs, ys);
+            assert xsRest !! pairKMap(inversersionSetJoined(xs[0..k]+xs[k+1..], ys),k,1);
+            assert pairKMap(inversersionSetJoined(xs[0..k]+xs[k+1..], ys),k,1) == inversersionSetJoined(xs, ys) - xsRest;
+
+            // assert xsRest <= invs;
+            something(xs, ys, sxs, sys, k);
+            assert |JoinedWith(sxs, sys, 0)| == |JoinedWith(xs, ys, k)|;
+            assert |invs| == |xsRest| + |pairKMap(inversersionSetJoined(xs[0..k] + xs[k+1..], ys), k, 1)|;
+            assert |sortedInvs| == |sxsFirst| + |pairSetMap2(inversersionSetJoined(sxs[1..], sys), 1)|;
+            assert |xsRest| == |sxsFirst|;
+            PiecesEqual(xs, ys, sxs, sys, k);
+            assert |pairKMap(inversersionSetJoined(xs[0..k] + xs[k+1..], ys), k, 1)| == |pairSetMap2(inversersionSetJoined(sxs[1..], sys), 1)|;
+            assert |invs| == |sortedInvs|;
+            assert |inversersionSetJoined(xs, ys)| == |inversersionSetJoined(sxs, sys)|;
+        }
+        
+    }
+
+
+
+    method BruteForceCount(xs: seq<int>) returns (numInv: int)
+        requires |xs| > 1
+        ensures numInv == countInversion(xs)
+    {
+        ghost var inversions: set<(int, int)> := {};
+        numInv := 0;
+        for i := 0 to |xs|-1 
+            invariant 0 <= i <= |xs|-1
+            invariant inversions == inversionSetPartial(xs, i)
+            invariant numInv == |inversions|
+        {
+            // assert i <= |xs|-2;
+            ghost var inversionsRows: set<(int, int)> := {};
+            ghost var irc := 0;
+            ghost var oldnumInv := numInv;
+            for j := i+1 to |xs| 
+                invariant i <= |xs|-2
+                invariant i+1 <= j <= |xs|
+                invariant inversionSetRowPartial(xs, i, j) == inversionsRows
+                invariant |inversionsRows| == irc
+                invariant numInv == irc+oldnumInv
+            {
+                ghost var oldInversionRows := inversionsRows;
+                if xs[i] > xs[j] {
+                    numInv := numInv + 1;
+                    inversionsRows := inversionsRows + {(i,j)};
+                    irc := irc + 1;
+                }
+            }
+            inversions := inversions + inversionsRows;
+        }
+        assert inversions == inversionSet(xs);
+    }
+
+// //Tim Roughgarden's algorithms illuminated part 1 page 64
+    method {:verify } {:vcs_split_on_every_assert} SortAndCountInv(xs: seq<int>) returns (sortedXs: seq<int>, numInv: int)
+        ensures numInv == countInversion(xs)
+        ensures multiset(sortedXs) == multiset(xs)
+        ensures Sorted(sortedXs)
+    {
+        if |xs| <= 1 {
+            return xs, 0;
+        }else{
+            var n := |xs|;
+            var m := n/2;
+            var left := xs[0..m];
+            var right := xs[m..];
+            assert xs == left + right;
+            assert multiset(left + right) == multiset(xs);
+            var leftSorted, leftInv := SortAndCountInv(left);
+            assert multiset(leftSorted) == multiset(left);
+            var rightSorted, rightInv := SortAndCountInv(right);
+            assert multiset(rightSorted) == multiset(right);
+            var merged, splitInv := MergeAndCountInv(leftSorted, rightSorted);
+            // assert multiset(merged) == multiset(left + right);
+            // assert multiset(merged) == multiset(leftSorted + rightSorted);
+            // assert multiset(merged) == multiset(xs);
+            inverionsetConcat(left, right);
+            inverionsetConcatSizes(left, right);
+            assert countInversion(left+right) == countInversion(left) + |pairSetMap(inversionSet(right), |left|)| + |inversersionSetJoined(left, right)|;
+            assert countInversion(left+right) == countInversion(xs);
+            assert leftInv == countInversion(left);
+            assert rightInv == countInversion(right);
+            inversetConcatOrderedUnorderedSame(left, right, leftSorted, rightSorted);
+            assert splitInv == |inversersionSetJoined(leftSorted, rightSorted)|;
+            assert splitInv == |inversersionSetJoined(left, right)|;
+            pairMapSize(right, |left|);
+            assert countInversion(left+right) == leftInv + rightInv + splitInv;
+            return merged, leftInv + rightInv + splitInv;
         }
     }
 
-//     lemma {:verify false}JoinedWith2MS(xs: seq<int>, ys: seq<int>, k: int, i: int)
-//         requires xs != []
-//         requires 0 <= k < |xs|
-//         requires 0 <= i < |ys|
-//         ensures IsInverted(xs+ys, k, |xs|+i) ==> |JoinedWith2(xs, ys, k)| == |JoinedWith2(xs, ys[0..i] + ys[i+1..], k)| + 1
-//         ensures !IsInverted(xs+ys, k, |xs|+i) ==> |JoinedWith2(xs, ys, k)| == |JoinedWith2(xs, ys[0..i] + ys[i+1..], k)|
-//     {
-//         if |ys| == 0 {
-
-//         }else if |ys| == 1 {
-
-//         }else{
-//             assert ys == ys[0..i] + [ys[i]] + ys[i+1..];
-//             if !IsInverted(xs+ys, k, |xs|+i) {
-
-//                 assert |JoinedWith2(xs, ys, k)| == |JoinedWith2(xs, ys[0..i] + ys[i+1..], k)|;
-//             }else{
-//                 assert |JoinedWith2(xs, ys, k)| == |JoinedWith2(xs, ys[0..i] + ys[i+1..], k)| + 1;
-
-//             }
-//         }
-//     }
-   
-
-//     lemma {:verify } JoinedWith2CardinalityEqualForOrderedAndUnordedSeqs(xs: seq<int>, ys: seq<int>, sxs: seq<int>, sys: seq<int>, k: int)
-//         requires xs != []
-//         requires 0 <= k < |xs|
-//         requires multiset(xs) == multiset(sxs)
-//         requires multiset(ys) == multiset(sys)
-//         requires Sorted(sxs)
-//         requires Sorted(sys)
-//         requires sxs[0] == xs[k]
-//         // decreases ys
-//         ensures |JoinedWith2(sxs, sys, 0)| == |JoinedWith2(xs, ys, k)|
-//     {
-//         if ys == [] {
-//             assert multiset(ys) == multiset([]);
-//             assert JoinedWith2(sxs, sys, 0) == {};
-//             assert JoinedWith2(xs, ys, k) == {};
-//             assert |JoinedWith2(sxs, sys, 0)| == |JoinedWith2(xs, ys, k)|;
-//         }else{
-//             if IsInverted(xs+ys, k, |xs|) {
-//                 assert ys == [ys[0]] + ys[1..];
-//                 assert multiset(ys) == multiset([ys[0]]) + multiset(ys[1..]);
-//                 assert ys[0] == (xs+ys)[|xs|];
-//                 assert ys[0] in multiset(ys);
-//                 assert ys[0] in sys;
-//                 var j :| 0 <= j < |sys| && ys[0] == sys[j];
-//                 assert sys == sys[0..j] + [ys[0]] + sys[j+1..];
-//                 assert multiset(sys) == multiset(sys[0..j]) + multiset([ys[0]]) + multiset(sys[j+1..]);
-//                 calc {
-//                     multiset(ys[1..]);
-//                     multiset(ys)-multiset{ys[0]};
-//                     multiset(sys)-multiset{ys[0]};
-//                 }
-//                 assert multiset(ys[1..]) == multiset(sys[0..j] + sys[j+1..]);
-//                 assert (sxs+sys)[0] == xs[k];
-//                 assert (sxs+sys)[|sxs|+j] == ys[0];
-//                 assert IsInverted(sxs+sys, 0, |sxs|+j);
-//                 JoinedWith2CardinalityEqualForOrderedAndUnordedSeqs(xs, ys[1..], sxs, sys[0..j] + sys[j+1..], k);
-//                 assert (k, |xs|) in JoinedWith2(xs, ys, k);
-//                 JoinedWithSame(sxs, sys, 0);
-//                 assert (0, |sxs|+j) in JoinedWith(sxs, sys, 0);
-//                 assert (0, |sxs|+j) in JoinedWith2(sxs, sys, 0);
-//                 JoinedWith2MS(sxs, sys, 0, j);
-//                 assert |JoinedWith2(sxs, sys, 0)| == 1 + |JoinedWith2(sxs, sys[0..j] + sys[j+1..], 0)|;
-
-//                 pairSetRmapLemma(JoinedWith2(xs, ys[1..], k), 1);
-//                 JoinedWith2Size(xs, ys, k);
-//                 assert |JoinedWith2(xs, ys[1..], k)| == |pairSetRmap(JoinedWith2(xs, ys[1..], k), 1)|;
-//                 assert JoinedWith2(xs, ys, k) == {(k, |xs|)}+pairSetRmap(JoinedWith2(xs, ys[1..], k), 1);
-//                 assert |JoinedWith2(xs, ys, k)| == 1+|pairSetRmap(JoinedWith2(xs, ys[1..], k), 1)|;
-//                 assert |JoinedWith2(xs, ys, k)| == 1 + |JoinedWith2(xs, ys[1..], k)|;
-//             assert |JoinedWith2(sxs, sys, 0)| == |JoinedWith2(xs, ys, k)|;
-//             }else{
-
-//                 assert ys == [ys[0]] + ys[1..];
-//                 assert multiset(ys) == multiset([ys[0]]) + multiset(ys[1..]);
-//                 assert ys[0] in multiset(ys);
-//                 assert ys[0] in sys;
-//                 var j :| 0 <= j < |sys| && ys[0] == sys[j];
-//                 assert sys == sys[0..j] + [ys[0]] + sys[j+1..];
-//                 assert multiset(sys) == multiset(sys[0..j]) + multiset([ys[0]]) + multiset(sys[j+1..]);
-//                 calc {
-//                     multiset(ys[1..]);
-//                     multiset(ys)-multiset{ys[0]};
-//                     multiset(sys)-multiset{ys[0]};
-//                 }
-//                 assert multiset(ys[1..]) == multiset(sys[0..j] + sys[j+1..]);
-//                 JoinedWith2CardinalityEqualForOrderedAndUnordedSeqs(xs, ys[1..], sxs, sys[0..j] + sys[j+1..], k);
-//                 JoinedWith2MS(sxs, sys, 0, j);
-//                 pairSetRmapLemma(JoinedWith2(xs, ys[1..], k), 1);
-//                 JoinedWith2Size(xs, ys, k);
-//                 assert |JoinedWith2(xs, ys, k)| == |JoinedWith2(xs, ys[1..], k)|;
-//             assert |JoinedWith2(sxs, sys, 0)| == |JoinedWith2(xs, ys, k)|;
-
-//             }
-//         }
-//     }
-
-//     lemma {:verify } something(xs: seq<int>, ys: seq<int>, sxs: seq<int>, sys: seq<int>, k: int)
-//         requires xs != []
-//         requires 0 <= k < |xs|
-//         requires multiset(xs) == multiset(sxs)
-//         requires multiset(ys) == multiset(sys)
-//         requires Sorted(sxs)
-//         requires Sorted(sys)
-//         requires sxs[0] == xs[k]
-//         ensures |JoinedWith(sxs, sys, 0)| == |JoinedWith(xs, ys, k)|
-//     {
-//         JoinedWith2CardinalityEqualForOrderedAndUnordedSeqs(xs, ys, sxs, sys, k);
-//         JoinedWithSame(sxs, sys, 0);
-//         JoinedWithSame(xs, ys, k);
-
-//     }
-
-//     lemma {:verify false} {:vcs_split_on_every_assert} inversetConcatOrderedUnorderedSame(xs: seq<int>, ys: seq<int>, sxs: seq<int>, sys: seq<int>)
-//         requires multiset(xs) == multiset(sxs)
-//         requires multiset(ys) == multiset(sys)
-//         requires Sorted(sxs)
-//         requires Sorted(sys)
-//         ensures |inversersionSetJoined(xs, ys)| == |inversersionSetJoined(sxs, sys)|
-//     {
-//         var n := |xs| + |ys|;
-//         var xsys := xs + ys;
-//         assert |xsys| == n;
-//         var sxsys := sxs + sys;
-//         seqMsLength(xs, sxs);
-//         seqMsLength(ys, sys);
-//         assert |sxsys| == n;
-//         assert multiset(xsys) == multiset(sxsys);
-//         var invs := inversersionSetJoined(xs, ys);
-//         if sxs == [] {
-
-//         }else {
-//             var x := sxs[0];
-//             assert sxs == [x] + sxs[1..];
-//             assert x in multiset(xs);
-//             var k :| 0 <= k < |xs| && x == xs[k];
-//             assert xs == xs[0..k] + [x] + xs[k+1..];
-//             assert multiset(xs) == multiset(xs[0..k] + [x] + xs[k+1..]);
-//             calc {
-//                 multiset(sxs[1..]);
-//                 multiset(sxs)-multiset{x};
-//                 multiset(xs)-multiset{x};
-//                 multiset(xs[0..k] + xs[k+1..]);
-//             }
-//             assert multiset(xs[0..k] + xs[k+1..]) == multiset(sxs[1..]);
-//             inversetConcatOrderedUnorderedSame(xs[0..k] + xs[k+1..], ys, sxs[1..], sys);
-//             assert |inversersionSetJoined(xs[0..k] + xs[k+1..], ys)| == |inversersionSetJoined(sxs[1..], sys)|;
-//             var sortedInvs := inversersionSetJoined(sxs, sys);
-//             var sxsFirst := JoinedWith(sxs, sys, 0);
-//             inversersionSetJoinedFirsts(sxs, sys);
-//             assert sxsFirst <= sortedInvs;
-//             // assume sxsFirst !! pairSetMap2(inversersionSetJoined(sxs[1..], sys), 1);
-//             assert sxsFirst + pairSetMap2(inversersionSetJoined(sxs[1..], sys),1) == inversersionSetJoined(sxs, sys);
-//             assert sxsFirst !! pairSetMap2(inversersionSetJoined(sxs[1..], sys),1) by {
-//                 forall pair | pair in pairSetMap2(inversersionSetJoined(sxs[1..], sys), 1)
-//                     ensures pair.0 != 0
-//                 {
-//                     pairSetMap2Inverse(inversersionSetJoined(sxs[1..], sys), 1, pair);
-//                 }
-//             }
-//             assert pairSetMap2(inversersionSetJoined(sxs[1..], sys), 1) == inversersionSetJoined(sxs, sys) - sxsFirst;
-//             var xsRest := JoinedWith(xs, ys, k);
-//             inversionSetJoinedMiddle2(xs, ys, k);
-//             assert xsRest + pairKMap(inversersionSetJoined(xs[0..k]+xs[k+1..], ys),k,1) == inversersionSetJoined(xs, ys);
-//             assert xsRest !! pairKMap(inversersionSetJoined(xs[0..k]+xs[k+1..], ys),k,1);
-//             assert pairKMap(inversersionSetJoined(xs[0..k]+xs[k+1..], ys),k,1) == inversersionSetJoined(xs, ys) - xsRest;
-
-//             // assert xsRest <= invs;
-//             something(xs, ys, sxs, sys, k);
-//             assert |JoinedWith(sxs, sys, 0)| == |JoinedWith(xs, ys, k)|;
-//             assert |invs| == |xsRest| + |pairKMap(inversersionSetJoined(xs[0..k] + xs[k+1..], ys), k, 1)|;
-//             assert |sortedInvs| == |sxsFirst| + |pairSetMap2(inversersionSetJoined(sxs[1..], sys), 1)|;
-//             // assume |pairKMap(inversersionSetJoined(xs[0..k] + xs[k+1..], ys), k, 1)| ==  |pairSetMap2(inversersionSetJoined(sxs[1..], sys), 1)|;
-
-//             assert |inversersionSetJoined(xs, ys)| == |inversersionSetJoined(sxs, sys)|;
-//         }
-        
-//     }
 
 
+    method {:verify }  MergeAndCountInv(left: seq<int>, right: seq<int>) returns (merged: seq<int>, splitInv: int)
+        requires Sorted(left)
+        requires Sorted(right)
+        ensures |merged| == |left| + |right|
+        ensures multiset(merged) == multiset(left + right)
+        // ensures splitInv == countInversion(merged)
+        ensures splitInv == |inversersionSetJoined(left, right)|
+        ensures Sorted(merged)
+    {
+        var n := |left| + |right|;
+        var i := 0;
+        var j := 0;
+        var k := 0;
+        ghost var inversions := inversersionSetJoined(left[0..i], right[0..j]);
+        assert inversions == {};
+        var inv := 0;
+        merged := [];
+        while k < n
+            invariant 0 <= k <= n
+            invariant k == i+j
+            invariant 0 <= i+j <= n
+            invariant 0 <= i <= |left|
+            invariant 0 <= j <= |right|
+            invariant |merged| == k
+            // invariant inversions == inversersionSetJoined(left[0..i], right[0..j])
+            // invariant inv == countInversion(merged)
+            invariant multiset(merged) == multiset(left[0..i] + right[0..j])
 
-//     method BruteForceCount(xs: seq<int>) returns (numInv: int)
-//         requires |xs| > 1
-//         ensures numInv == countInversion(xs)
-//     {
-//         ghost var inversions: set<(int, int)> := {};
-//         numInv := 0;
-//         for i := 0 to |xs|-1 
-//             invariant 0 <= i <= |xs|-1
-//             invariant inversions == inversionSetPartial(xs, i)
-//             invariant numInv == |inversions|
-//         {
-//             // assert i <= |xs|-2;
-//             ghost var inversionsRows: set<(int, int)> := {};
-//             ghost var irc := 0;
-//             ghost var oldnumInv := numInv;
-//             for j := i+1 to |xs| 
-//                 invariant i <= |xs|-2
-//                 invariant i+1 <= j <= |xs|
-//                 invariant inversionSetRowPartial(xs, i, j) == inversionsRows
-//                 invariant |inversionsRows| == irc
-//                 invariant numInv == irc+oldnumInv
-//             {
-//                 ghost var oldInversionRows := inversionsRows;
-//                 if xs[i] > xs[j] {
-//                     numInv := numInv + 1;
-//                     inversionsRows := inversionsRows + {(i,j)};
-//                     irc := irc + 1;
-//                 }
-//             }
-//             inversions := inversions + inversionsRows;
-//         }
-//         assert inversions == inversionSet(xs);
-//     }
+            // invariant forall x :: 0 <= x < |merged| ==> merged[x] <= right[j];
+            invariant forall x :: x in merged ==> x in left[..i] || x in right[..j]
+            invariant forall x, y :: x in merged && y in left[i..]+right[j..] ==> x <= y
+            invariant Sorted(merged)
+            invariant inv == |inversersionSetJoined(left, right[0..j])|
+        {
+            assert left == left[0..i] + left[i..];
+            assert right == right[0..j] + right[j..];
+            print "before: i: ",i," j: ",j, " inv: ", inv," ", inversersionSetJoined(left, right[..j]), " |_|=", |inversersionSetJoined(left, right[..j])|, "\n";
+            InversionSetJoinMaintained(left, right, i, j, inv, merged);
+            if j >= |right| || (i < |left| && left[i] <= right[j]) {
+                assert i < |left| by {
+                    if i < |left| {
+                        assert i < |left|;
+                    }else{
+                        assert j >= |right|;
+                    }
+                }
 
-// //Tim Roughgarden's algorithms illuminated part 1 page 64
-//     method {:verify } {:vcs_split_on_every_assert} SortAndCountInv(xs: seq<int>) returns (sortedXs: seq<int>, numInv: int)
-//         ensures numInv == countInversion(xs)
-//         ensures multiset(sortedXs) == multiset(xs)
-//         ensures Sorted(sortedXs)
-//     {
-//         if |xs| <= 1 {
-//             return xs, 0;
-//         }else{
-//             var n := |xs|;
-//             var m := n/2;
-//             var left := xs[0..m];
-//             var right := xs[m..];
-//             assert xs == left + right;
-//             assert multiset(left + right) == multiset(xs);
-//             var leftSorted, leftInv := SortAndCountInv(left);
-//             assert multiset(leftSorted) == multiset(left);
-//             var rightSorted, rightInv := SortAndCountInv(right);
-//             assert multiset(rightSorted) == multiset(right);
-//             var merged, splitInv := MergeAndCountInv(leftSorted, rightSorted);
-//             // assert multiset(merged) == multiset(left + right);
-//             // assert multiset(merged) == multiset(leftSorted + rightSorted);
-//             // assert multiset(merged) == multiset(xs);
-//             inverionsetConcat(left, right);
-//             inverionsetConcatSizes(left, right);
-//             assert countInversion(left+right) == countInversion(left) + |pairSetMap(inversionSet(right), |left|)| + |inversersionSetJoined(left, right)|;
-//             assert countInversion(left+right) == countInversion(xs);
-//             assert leftInv == countInversion(left);
-//             assert rightInv == countInversion(right);
-//             inversetConcatOrderedUnorderedSame(left, right, leftSorted, rightSorted);
-//             assert splitInv == |inversersionSetJoined(leftSorted, rightSorted)|;
-//             assert splitInv == |inversersionSetJoined(left, right)|;
-//             pairMapSize(right, |left|);
-//             assert countInversion(left+right) == leftInv + rightInv + splitInv;
-//             return merged, leftInv + rightInv + splitInv;
-//         }
-//     }
-
-//     method {:verify false} {:vcs_split_on_every_assert} MergeAndCountInv(left: seq<int>, right: seq<int>) returns (merged: seq<int>, splitInv: int)
-//         requires Sorted(left)
-//         requires Sorted(right)
-//         ensures |merged| == |left| + |right|
-//         ensures multiset(merged) == multiset(left + right)
-//         // ensures splitInv == countInversion(merged)
-//         ensures splitInv == |inversersionSetJoined(left, right)|
-//         ensures Sorted(merged)
-//     {
-//         var n := |left| + |right|;
-//         var i := 0;
-//         var j := 0;
-//         var k := 0;
-//         ghost var inversions := inversersionSetJoined(left[0..i], right[0..j]);
-//         assert inversions == {};
-//         var inv := 0;
-//         merged := [];
-//         while k < n
-//             invariant 0 <= k <= n
-//             invariant k == i+j
-//             invariant 0 <= i+j <= n
-//             invariant 0 <= i <= |left|
-//             invariant 0 <= j <= |right|
-//             invariant |merged| == k
-//             // invariant inv == countInversion(merged)
-//             invariant multiset(merged) == multiset(left[0..i] + right[0..j])
-//             invariant forall x :: x in merged ==> x in left[..i] || x in right[..j]
-//             invariant forall x, y :: x in merged && y in left[i..]+right[j..] ==> x <= y
-//             invariant Sorted(merged)
-//             invariant inv == |inversersionSetJoined(left[0..i], right[0..j])|
-//         {
-//             assert left == left[0..i] + left[i..];
-//             assert right == right[0..j] + right[j..];
-//             if j >= |right| || (i < |left| && left[i] < right[j]) {
-//                 assert i < |left| by {
-//                     if i < |left| {
-//                         assert i < |left|;
-//                     }else{
-//                         assert j >= |right|;
-//                     }
-//                 }
-
-//                 // assert Sorted(merged); 
-//                 assert forall x, y :: x in merged && y in left[i..]+right[j..] ==> x <= y;
-//                 assert left[i] in left[i..]+right[j..];
-//                 assert forall x :: 0 <= x < |merged| ==> merged[x] <= left[i] by {
-//                     forall x | 0 <= x < |merged|
-//                         ensures merged[x] <= left[i]
-//                     {
+                // assert Sorted(merged); 
+                assert forall x, y :: x in merged && y in left[i..]+right[j..] ==> x <= y;
+                assert left[i] in left[i..]+right[j..];
+                assert forall x :: 0 <= x < |merged| ==> merged[x] <= left[i] by {
+                    forall x | 0 <= x < |merged|
+                        ensures merged[x] <= left[i]
+                    {
                         
-//                         assert merged[x] in merged;
-//                     }
-//                 }
-//                 ghost var oldmerged := merged;
-//                 merged := merged + [left[i]];
-//                 assert left[0..i+1] == left[0..i] + [left[i]];
-//                 assert multiset(merged) == multiset(left[0..i+1] + right[0..j]);
-//                 assert forall x, y :: x in merged && y in left[i+1..]+right[j..] ==> x <= y by {
-//                     forall x, y | x in merged && y in left[i+1..]+right[j..] 
-//                         ensures x <= y
-//                     {
-//                         if x in left[0..i+1] {
-//                             assert x <= left[i];
-//                             assert x <= y;
-//                         }else{
-//                             assert x in merged;
-//                             assert x in right[0..j];
-//                             var k :| 0 <= k < j <= |right| && x == right[k];
-//                             assert k < j;
-//                             if y in left[i+1..] {
-//                                 assert y >= left[i]; 
-//                                 if x == left[i] {
-//                                     assert x <= left[i];
-//                                 }else if x in oldmerged {
-//                                     assert forall z, w :: z in oldmerged && w in left[i..]+right[j..] ==> z <= w; 
-//                                     assert left[i] in left[i..]+right[j..];
-//                                     assert x <= left[i];
+                        assert merged[x] in merged;
+                    }
+                }
+                ghost var oldmerged := merged;
+                merged := merged + [left[i]];
+                assert left[0..i+1] == left[0..i] + [left[i]];
+                assert multiset(merged) == multiset(left[0..i+1] + right[0..j]);
+                assert forall x, y :: x in merged && y in left[i+1..]+right[j..] ==> x <= y by {
+                    forall x, y | x in merged && y in left[i+1..]+right[j..] 
+                        ensures x <= y
+                    {
+                        if x in left[0..i+1] {
+                            assert x <= left[i];
+                            assert x <= y;
+                        }else{
+                            assert x in merged;
+                            assert x in right[0..j];
+                            var k :| 0 <= k < j <= |right| && x == right[k];
+                            assert k < j;
+                            if y in left[i+1..] {
+                                assert y >= left[i]; 
+                                if x == left[i] {
+                                    assert x <= left[i];
+                                }else if x in oldmerged {
+                                    assert forall z, w :: z in oldmerged && w in left[i..]+right[j..] ==> z <= w; 
+                                    assert left[i] in left[i..]+right[j..];
+                                    assert x <= left[i];
 
-//                                 }
-//                                 assert x <= y;
-//                             }else{
-//                                 assert y in right[j..];
-//                                 assert x <= y;
+                                }
+                                assert x <= y;
+                            }else{
+                                assert y in right[j..];
+                                assert x <= y;
 
-//                             }
-//                         }
-//                     }
-//                 }
-//                 // assert Sorted(merged) by {
-//                 //     forall i,j | 0 <= i < j < |merged| 
-//                 //         ensures merged[i] <= merged[j];
-//                 //     {
-                        
-//                 //     }
-//                 // }
-//                 i := i + 1;
-//             }else{
-//                 assume forall x :: 0 <= x < |merged| ==> merged[x] <= right[j];
-//                 assert right[0..j+1] == right[0..j] + [right[j]];
-//                 merged := merged + [right[j]];
-//                 assert forall x, y :: x in merged && y in left[i..]+right[j+1..] ==> x <= y;
-//                 j := j + 1;
-//                 assert Sorted(merged);
-//                 inv := inv + |left| - i;
-//             }
-//             k := k + 1;
+                            }
+                        }
+                    }
+                }
+                i := i + 1;
+                assert inv == |inversersionSetJoined(left, right[0..j])|;
+            }else{
+                // assume forall x :: 0 <= x < |merged| ==> merged[x] <= right[j];
+                assert forall x :: 0 <= x < |merged| ==> merged[x] <= right[j] by {
+                    assert right[j] in left[i..]+right[j..];
+                    forall x | 0 <= x < |merged|
+                        ensures merged[x] <= right[j]
+                    {
+                        assert merged[x] in merged;
 
-//             assume inv == |inversersionSetJoined(left[0..i], right[0..j])|;
-//         }
-//         assert i == |left|;
-//         assert j == |right|;
-//         assert left[0..i] == left;
-//         assert right[0..j] == right;
-//         assert multiset(left[0..i]) == multiset(left);
-//         assert multiset(merged) == multiset(left + right);
-//         return merged, inv;
-//     }
+                    }
+                }
+                assert right[0..j+1] == right[0..j] + [right[j]];
+                merged := merged + [right[j]];
+                assert forall x, y :: x in merged && y in left[i..]+right[j+1..] ==> x <= y;
+                j := j + 1;
+                assert Sorted(merged);
+                inv := inv + |left| - i;
+                assert inv == |inversersionSetJoined(left, right[0..j])|;
+            }
+            k := k + 1;
+            print "after: i: ",i," j: ",j, " inv: ", inv," ", inversersionSetJoined(left, right[..j]), " |_|=", |inversersionSetJoined(left, right[..j])|, "\n";
+
+            // assume inv == |inversersionSetJoined(left[0..i], right[0..j])|;
+        }
+        assert i == |left|;
+        assert j == |right|;
+        assert left[0..i] == left;
+        assert right[0..j] == right;
+        assert multiset(left[0..i]) == multiset(left);
+        assert multiset(merged) == multiset(left + right);
+        return merged, inv;
+    }
+
+    method Main() {
+        var res1, rest := SortAndCountInv([1,2,5,6,7]+[7,8]);
+        print res1;
+        print rest;
+    }
 }
